messageInvariantPrototypes/clientServer/applicationProof.dfy
@@ -1,0 +1,48 @@
+include "spec.dfy"
+include "messageInvariants.dfy"
+
+module ClientServerProof {
+import opened Types
+import opened UtilitiesLibrary
+import opened DistributedSystem
+import opened Obligations
+import opened MessageInvariants
+  
+
+/***************************************************************************************
+*                                Application Invariants                                *
+***************************************************************************************/
+
+// There are no application invariants :)
+
+predicate Inv(c: Constants, v: Variables)
+{
+  && MessageInv(c, v)
+  && Safety(c, v)
+}
+
+/***************************************************************************************
+*                                        Proof                                         *
+***************************************************************************************/
+
+lemma InvImpliesSafety(c: Constants, v: Variables)
+  requires Inv(c, v)
+  ensures Safety(c, v)
+{}
+
+lemma InitImpliesInv(c: Constants, v: Variables)
+  requires Init(c, v)
+  ensures Inv(c, v)
+{
+  InitImpliesMessageInv(c, v);
+}
+
+lemma InvInductive(c: Constants, v: Variables, v': Variables)
+  requires Inv(c, v)
+  requires Next(c, v, v')
+  ensures Inv(c, v')
+{
+  MessageInvInductive(c, v, v');
+}
+}  // end module ClientServerProof
+
