messageInvariantPrototypes/clientServer/messageInvariants.dfy
@@ -1,0 +1,65 @@
+include "spec.dfy"
+
+module MessageInvariants {
+
+import opened Types
+import opened UtilitiesLibrary
+import opened DistributedSystem
+import opened Obligations
+
+// certified self inductive, modulo requires
+predicate RequestsValidSource(c: Constants, v: Variables) 
+  requires v.WF(c)
+{
+  forall req | req in v.network.sentMsgs && req.Request?
+  :: c.ValidClientIdx(req.clientId)
+}
+
+// certified self inductive, modulo requires
+predicate ResponseCorrespondToRequest(c: Constants, v: Variables)
+  requires v.WF(c)
+{
+  forall resp | resp in v.network.sentMsgs && resp.Response?
+  :: Request(resp.clientId, resp.reqId) in v.network.sentMsgs
+}
+
+// certified self inductive, modulo requires
+predicate RequestMessagesValid(c: Constants, v: Variables)
+  requires v.WF(c)
+  requires RequestsValidSource(c, v)
+{
+  forall req | req in v.network.sentMsgs && req.Request?
+  :: req.reqId in v.hosts[req.clientId].client.requests
+}
+
+// certified self inductive, modulo requires
+predicate ReceivedResponsesValid(c: Constants, v: Variables)
+  requires v.WF(c)
+{
+  forall idx:nat, respId | c.ValidClientIdx(idx) && respId in v.hosts[idx].client.responses
+  :: Response(idx, respId) in v.network.sentMsgs
+}
+
+
+predicate MessageInv(c: Constants, v: Variables) 
+{
+  && v.WF(c)
+  && RequestsValidSource(c, v)
+  && ResponseCorrespondToRequest(c, v)
+  && RequestMessagesValid(c, v)
+  && ReceivedResponsesValid(c, v)
+}
+
+lemma InitImpliesMessageInv(c: Constants, v: Variables)
+  requires Init(c, v)
+  ensures MessageInv(c, v)
+{}
+
+lemma MessageInvInductive(c: Constants, v: Variables, v': Variables)
+  requires MessageInv(c, v)
+  requires Next(c, v, v')
+  ensures MessageInv(c, v')
+{}
+
+}  // end module MessageInvariants
+
