messageInvariantPrototypes/clientServer/types.dfy
@@ -1,0 +1,12 @@
+include "../lib/UtilitiesLibrary.dfy"
+
+module Types {
+  import opened UtilitiesLibrary
+
+  type ClientId = nat
+  
+  datatype Message =
+    Request(clientId: ClientId, reqId: nat) | Response(clientId: ClientId, reqId: nat)
+
+  datatype MessageOps = MessageOps(recv:Option<Message>, send:Option<Message>)
+} // end module Types
