messageInvariantPrototypes/clientServer/readme.md
@@ -1,3 +1,3 @@
-This is the "client_server_ae" protocol from [DuoAI](https://github.com/VeriGu/DuoAI/tree/master/protocols). 
+This is the "client_server_ae" protocol from [DuoAI](https://github.com/VeriGu/DuoAI/tree/master/protocols) (OSDI'22). 
 
-This protocol is rather simple --- there are no application 
+Multiple clients can send requests to a server. The server processes each request and returns a response to the respective client. The server may process the requests out-of-order.
